Test_Variables.thy
@@ -1,0 +1,44 @@
+theory Test_Variables
+  imports Variables
+begin
+
+record memory = mem_x :: int   mem_y :: "int"   mem_z :: nat
+
+(* TODO: Should be possible to declare many variables in one go,
+    together with independence theorems *)
+declare_variable x get "mem_x" set "\<lambda>a m. m\<lparr>mem_x := a\<rparr>"
+  by auto
+
+declare_variable y get "mem_y" set "\<lambda>a m. m\<lparr>mem_y := a\<rparr>"
+  by auto
+
+declare_variable z get "mem_z" set "\<lambda>a m. m\<lparr>mem_z := a\<rparr>"
+  by auto
+
+lemma [simp, independence]:
+  "independent_vars x y" "independent_vars y x"
+  "independent_vars x z" "independent_vars z x"
+  "independent_vars y z" "independent_vars z y"
+  unfolding independent_vars_def by simp_all
+
+lemma [simp]:
+  "independent_of mem_x y" "independent_of mem_y x"
+  "independent_of mem_x z" "independent_of mem_z x"
+  "independent_of mem_y z" "independent_of mem_z y"
+  unfolding independent_of_def by simp_all
+
+
+
+(* Test *)
+
+
+lemma
+  "independent_vars x y" "independent_vars y x"
+  "independent_vars x z" "independent_vars z x"
+  "independent_vars y z" "independent_vars z y"
+  "independent_of mem_x y" "independent_of mem_y x"
+  "independent_of mem_x z" "independent_of mem_z x"
+  "independent_of mem_y z" "independent_of mem_z y"
+  by simp_all
+
+end
