Utils.thy
@@ -1,0 +1,7 @@
+theory Utils
+  imports Main
+begin
+
+ML_file "utils.ML"
+
+end
